dllbc/Dllbc.lean
@@ -34,4 +34,5 @@ import Dllbc.Tests.AmbiguousMiddle
 import Dllbc.Tests.MatchJoin
 import Dllbc.StdChain
 import Dllbc.Tests.ModuleStates
+import Dllbc.Tests.Parse
 
